src/tests/tactics.fs
@@ -4,23 +4,28 @@ open FStar
 open FStar.Util
 open FStar.Syntax.Syntax
 open FStar.Tests.Pars
-module S = FStar.Syntax.Syntax
-module U = FStar.Syntax.Util
+module S  = FStar.Syntax.Syntax
+module U  = FStar.Syntax.Util
 module SS = FStar.Syntax.Subst
-module I = FStar.Ident
+module I  = FStar.Ident
 module P  = FStar.Syntax.Print
+module N  = FStar.TypeChecker.Normalize
 open FStar.Ident
 open FStar.Range
 open FStar.Tests.Util
 open FStar.Tactics.Basic
 
-let g1 =  {
-    context=snd (Pars.init());
-    goal_ty= Pars.tc "forall (x:int). x==0 \
+let g1 =
+    let env = snd (Pars.init()) in
+    let tm = Pars.tc "forall (x:int). x==0 \
                             ==> (forall (y:int). y==0 \
-                                             ==> x==y)";
-    witness=None
-}
+                                             ==> x==y)" in
+    let tm = N.normalize [N.Beta] env tm in
+    {
+      context=env;
+      goal_ty=tm;
+      witness=None
+    }
 
 let proofstate_of_goal g = {
     main_context=snd (Pars.init());
@@ -29,13 +34,14 @@ let proofstate_of_goal g = {
     goals=[g];
     transaction=Unionfind.new_transaction()
 }
-  
-let test () = 
+
+let test () =
+    FStar.Main.process_args() |> ignore; //set the command line args for debugging
+    printfn "Goal is %s" (P.term_to_string g1.goal_ty);
     let p1 = proofstate_of_goal g1 in
-    match simplify_eq_impl p1 with
-    | Success (_, p2) -> 
+    match FStar.Tactics.Basic.visit_strengthen simplify_eq_impl p1 with
+    | Success (_, p2) ->
       p2.goals |> List.iter (fun g ->
       printfn "Goal: %s" (P.term_to_string g.goal_ty))
     | Failed (msg, _) ->
-      printfn "Tactic failed: %s" msg                                    
- 
+      printfn "Tactic failed: %s" msg
